{
 "cells": [
  {
   "cell_type": "markdown",
   "id": "29cb8183",
   "metadata": {},
   "source": [
    "## Curious: Where do the expressions for the up and down factors come from in the CRR model?\n",
    "In the CRR model the $u$ and $d$ are based on the volatility $\\sigma$ of the underlying asset, the time step $\\Delta{t}$ and the symmetric condition $ud = 1$:\n",
    "$$\\begin{align*}\n",
    "u & = e^{\\sigma\\sqrt{\\Delta{t}}} \\\\\n",
    "d & = e^{-\\sigma\\sqrt{\\Delta{t}}}\n",
    "\\end{align*}$$\n",
    "where $\\sigma$ is the implied volatility of the growth rate (return) of the underlying asset. But where do these expressions come from?\n",
    "___"
   ]
  },
  {
   "cell_type": "markdown",
   "id": "09ace64f",
   "metadata": {},
   "source": [
    "## Derivation\n",
    "The CRR model matches the volatility of the binomial model to that of geometric Brownian motion (GBM). In the binomial model, if the stock moves up by a factor $u$ or down by a factor $d$, the log-return over one step is:\n",
    "$$\n",
    "\\ln\\frac{S(t+\\Delta t)}{S(t)} = \n",
    "\\begin{cases}\n",
    "\\ln(u) = a & \\text{with probability } p,\\\\\n",
    "\\ln(d) = -a & \\text{with probability } 1-p,\n",
    "\\end{cases}\n",
    "$$\n",
    "where we define $a = \\ln(u)$ and use the symmetry condition $d = 1/u$, which gives $\\ln(d) = -a$. Let $X$ denote this log-return random variable:\n",
    "$$\n",
    "\\begin{align*}\n",
    "X & =\n",
    "\\begin{cases}\n",
    "+a & \\text{with probability } p,\\\\\n",
    "-a & \\text{with probability } 1-p.\n",
    "\\end{cases}\n",
    "\\end{align*}\n",
    "$$\n",
    "We want to match the variance of this two-point random variable $X$ to the variance of the GBM log-return. The mean of $X$ is:\n",
    "$$\n",
    "\\mathbb{E}[X] = p\\cdot(+a) + (1-p)\\cdot(-a) = (2p-1)a.\n",
    "$$\n",
    "The second moment is:\n",
    "$$\n",
    "\\mathbb{E}[X^2] = p\\cdot a^2 + (1-p)\\cdot a^2 = a^2.\n",
    "$$\n",
    "Using the variance formula $\\mathrm{Var}(X) = \\mathbb{E}[X^2] - (\\mathbb{E}[X])^2$, we have:\n",
    "$$\n",
    "\\mathrm{Var}(X)\n",
    "= \\mathbb{E}[X^2] - (\\mathbb{E}[X])^2\n",
    "= a^2 - \\big[(2p-1)a\\big]^2\n",
    "= a^2\\Big[1 - (2p-1)^2\\Big]\n",
    "= 4p(1-p)a^2.\n",
    "$$\n",
    "From the geometric Brownian motion model, the variance of the log return over time $\\Delta t$ is:\n",
    "$$\n",
    "\\mathrm{Var}\\Bigg[\\ln\\frac{S(t+\\Delta t)}{S(t)}\\Bigg]\n",
    "= \\sigma^2 \\Delta t.\n",
    "$$\n",
    "We set the binomial variance equal to the GBM variance:\n",
    "$$\n",
    "4p(1-p)a^2 = \\sigma^2 \\Delta t.\n",
    "$$\n",
    "At this point, CRR makes a simplifying choice: at the microscopic time scale $\\Delta t$, take the up/down moves to be balanced, i.e., $p = \\tfrac{1}{2}$. Plugging $p = \\tfrac{1}{2}$ gives:\n",
    "$$\n",
    "4\\cdot \\tfrac{1}{2}\\cdot\\tfrac{1}{2}a^2 = a^2 = \\sigma^2 \\Delta t.\n",
    "$$\n",
    "which yields:\n",
    "$$\n",
    "a^2 = \\sigma^2 \\Delta t\n",
    "\\quad\\Longrightarrow\\quad\n",
    "a = \\sigma\\sqrt{\\Delta t}.\n",
    "$$\n",
    "Recall that we defined $u = e^{a}$ and $d = e^{-a}$ from the symmetry condition $ud = 1$. Therefore:\n",
    "$$\n",
    "\\boxed{\n",
    "u = e^{+\\sigma\\sqrt{\\Delta t}},\n",
    "\\qquad\n",
    "d = e^{-\\sigma\\sqrt{\\Delta t}}.\n",
    "}\n",
    "$$\n",
    "That is exactly the Cox–Ross–Rubinstein form!"
   ]
  }
 ],
 "metadata": {
  "language_info": {
   "name": "python"
  }
 },
 "nbformat": 4,
 "nbformat_minor": 5
}
